coq/Completeness.v
@@ -11,17 +11,100 @@ From SE Require Import WellDefinedness.
 From SE.SMT Require Import Expr.
 From SE.SMT Require Import Model.
 
-Lemma completeness_single_step :
-  forall c c' s,
-    step c c' -> well_defined s -> over_approx s c -> (exists s', sym_step s s' /\ over_approx s' c').
+(* TODO: rename *)
+Lemma smt_lemma_1 : forall c_ls s_ls c_gs s_gs ot e m,
+    (forall (x : raw_id), equiv_via_model (c_ls x) (s_ls x) m) /\
+    (forall (x : raw_id), equiv_via_model (c_gs x) (s_gs x) m) /\
+    equiv_via_model (eval_exp c_ls c_gs ot e) (sym_eval_exp s_ls s_gs ot e) m.
 Proof.
 Admitted.
 
+Lemma completeness_single_step :
+  forall c c' s,
+    is_supported_state c ->
+    step c c' ->
+    well_defined s ->
+    over_approx s c ->
+    (exists s', sym_step s s' /\ over_approx s' c').
+Proof.
+  intros c c' s Hiss Hs Hwd Hoa.
+  destruct c as [c_ic c_c c_cs c_pbid c_ls c_stk c_gs c_mdl].
+  destruct s as [s_ic s_c s_cs s_pbid s_ls s_stk s_gs s_syms s_pc s_mdl].
+  inversion Hs; subst.
+  {
+    inversion Hoa; subst.
+    destruct H as [m H].
+    inversion H; subst.
+    assert(L :
+      equiv_via_model
+        (eval_exp c_ls c_gs None e)
+        (sym_eval_exp s_ls s_gs None e)
+        m
+    ).
+    { apply smt_lemma_1. }
+    inversion L; subst.
+    { simpl in H8. rewrite H8 in *. discriminate H1. }
+    {
+      exists (mk_sym_state
+        (next_inst_counter c_ic c)
+        c
+        cs
+        c_pbid
+        (v !-> Some se; s_ls)
+        s_stk
+        s_gs
+        s_syms
+        s_pc
+        c_mdl
+      ).
+      split.
+      {
+        apply Sym_Step_OP.
+        symmetry.
+        simpl.
+        assumption.
+      }
+      {
+        apply OA_State.
+        exists m.
+        apply OAV_State.
+        destruct H20 as [H20_1 [H20_2 H20_3]].
+        split.
+        {
+          intros x.
+          destruct (raw_id_eqb x v) eqn:E.
+          {
+            rewrite raw_id_eqb_eq in E.
+            rewrite E.
+            rewrite update_map_eq, update_map_eq.
+            rewrite H8 in H0.
+            rewrite <- H0.
+            apply EVM_Some.
+            assumption.
+          }
+          {
+            rewrite raw_id_eqb_neq in E.
+            rewrite update_map_neq, update_map_neq; try (symmetry; assumption).
+            apply H20_1.
+          }
+        }
+        {
+          split.
+          { apply H20_2. }
+          { assumption. }
+        }
+      }
+    }
+  }
+Admitted.
+
+(* TODO: add module preconditions *)
 Lemma completeness :
   forall (mdl : llvm_module) (d : llvm_definition) (c : state),
     exists init_c,
       (init_state mdl d) = Some init_c ->
       multi_step init_c c ->
-      (exists init_s s, (init_sym_state mdl d) = Some init_s /\ multi_sym_step init_s s /\ over_approx s c).
+      (exists init_s s,
+        (init_sym_state mdl d) = Some init_s /\ multi_sym_step init_s s /\ over_approx s c).
 Proof.
 Admitted.
